txn-data-consistency/Tapir_Falsification.thy
@@ -40,8 +40,7 @@ lemma commit_wr_abs_committed_reads_inv:
   shows
     "abs_committed_reads (s \<lparr>svrs := (svrs s)
       (k := svrs s k \<lparr>
-        svr_state := (svr_state (svrs s k)) (Tn t := committed a b c),
-        svr_ver_order := X\<rparr>)\<rparr>) k' t_wr =
+        svr_state := (svr_state (svrs s k)) (Tn t := committed a b c)\<rparr>)\<rparr>) k' t_wr =
      abs_committed_reads s k' t_wr"
   using assms
   by (auto simp add: abs_committed_reads_def)
@@ -71,47 +70,89 @@ lemma corder_sub_ext_corder:
   "t \<in> set (corder k) \<Longrightarrow> t \<in> set (ext_corder t wm corder k)"
   by (auto simp add: ext_corder_def)
 
-definition Svr_Ver_Ord_Non_Emp where
-  "Svr_Ver_Ord_Non_Emp s k \<longleftrightarrow> svr_ver_order (svrs s k) \<noteq> []"
+definition T0_Committed where
+  "T0_Committed s k \<longleftrightarrow> (is_committed_wr (svr_state (svrs s k) T0))"
                                                            
-lemmas Svr_Ver_Ord_Non_EmpI = Svr_Ver_Ord_Non_Emp_def[THEN iffD2, rule_format]
-lemmas Svr_Ver_Ord_Non_EmpE[elim] = Svr_Ver_Ord_Non_Emp_def[THEN iffD1, elim_format, rule_format]
+lemmas T0_CommittedI = T0_Committed_def[THEN iffD2, rule_format]
+lemmas T0_CommittedE[elim] = T0_Committed_def[THEN iffD1, elim_format, rule_format]
          
-lemma reach_svr_ver_ord_non_emp [simp, dest]: "reach tapir s \<Longrightarrow> Svr_Ver_Ord_Non_Emp s k"
+lemma reach_t0_committed [simp, dest]: "reach tapir s \<Longrightarrow> T0_Committed s k"
 proof(induction s rule: reach.induct)
   case (reach_init s)
   then show ?case
-  by (auto simp add: Svr_Ver_Ord_Non_Emp_def tapir_defs)
+  by (auto simp add: T0_Committed_def tapir_defs)
 next
   case (reach_trans s e s')
   then show ?case
-    by (induction e) (auto simp add: Svr_Ver_Ord_Non_Emp_def tapir_trans_defs)
+    by (induction e) (auto simp add: T0_Committed_def tapir_trans_defs)
 qed
 
-definition Svr_Ver_Ord_Cmt where
-  "Svr_Ver_Ord_Cmt s k \<longleftrightarrow> (\<forall>t \<in> set (svr_ver_order (svrs s k)).
-    (\<exists>ts rto v. svr_state (svrs s k) t = committed ts rto (Some v)))"
+definition Finite_Committed where
+  "Finite_Committed s k \<longleftrightarrow> (finite {t. is_committed_wr (svr_state (svrs s k) t)})"
                                                            
-lemmas Svr_Ver_Ord_CmtI = Svr_Ver_Ord_Cmt_def[THEN iffD2, rule_format]
-lemmas Svr_Ver_Ord_CmtE[elim] = Svr_Ver_Ord_Cmt_def[THEN iffD1, elim_format, rule_format]
+lemmas Finite_CommittedI = Finite_Committed_def[THEN iffD2, rule_format]
+lemmas Finite_CommittedE[elim] = Finite_Committed_def[THEN iffD1, elim_format, rule_format]
          
-lemma reach_svr_ver_ord_cmt [simp, dest]: "reach tapir s \<Longrightarrow> Svr_Ver_Ord_Cmt s k"
+lemma reach_finite_committed [simp, dest]: "reach tapir s \<Longrightarrow> Finite_Committed s k"
 proof(induction s rule: reach.induct)
   case (reach_init s)
   then show ?case
-  by (auto simp add: Svr_Ver_Ord_Cmt_def tapir_defs)
+  by (auto simp add: Finite_Committed_def tapir_defs)
 next
   case (reach_trans s e s')
   then show ?case
-    by (induction e) (auto simp add: Svr_Ver_Ord_Cmt_def tapir_trans_defs)
+  proof (induction e)
+    case (Prep x1 x2 x3 x4 x5a)
+    then show ?case
+      apply (simp add: Finite_Committed_def tapir_trans_defs)
+      by (smt (verit, best) Collect_cong is_committed_wr.elims(2) is_committed_wr.simps(3)
+          is_committed_wr.simps(6) occ_check_resE svr_state.distinct(15))
+  next
+    case (Commit x1 x2 x3 x4 x5a)
+    then have "finite (insert (Tn x2) {t. is_committed_wr (svr_state (svrs s k) t)})" by auto
+    then show ?case using Commit
+      by (auto simp add: Finite_Committed_def tapir_trans_defs insert_Collect)
+  qed (auto simp add: Finite_Committed_def tapir_trans_defs Collect_mono rev_finite_subset)
 qed
+
+definition Finite_Committed_Ts where
+  "Finite_Committed_Ts s k \<longleftrightarrow>
+    (finite {ts. \<exists>t. is_committed_wr (svr_state (svrs s k) t) \<and> ts = v_ts (svr_state (svrs s k) t)})"
+
+lemmas Finite_Committed_TsI = Finite_Committed_Ts_def[THEN iffD2, rule_format]
+lemmas Finite_Committed_TsE[elim] = Finite_Committed_Ts_def[THEN iffD1, elim_format, rule_format]
+         
+lemma reach_finite_committed_ts [simp, dest]: "reach tapir s \<Longrightarrow> Finite_Committed_Ts s k"
+  using Finite_Committed_def[of s] by (simp add: Finite_Committed_Ts_def)
+
+lemma arg_max_exI:
+  fixes f :: "'a \<Rightarrow> 'b :: linorder"
+  assumes "finite {y. \<exists>x. P x \<and> y = f x}" and "P t"
+  shows "\<exists>x. is_arg_max f P x"
+proof -
+  obtain x where "P x" "Max {y. \<exists>x. P x \<and> y = f x} = f x"
+    using Max_in assms by auto
+  then show ?thesis apply (simp add: is_arg_max_def)
+    by (smt Max_ge assms(1) leD mem_Collect_eq)
+qed
+
+definition Latest_Committed_Wtxn where
+  "Latest_Committed_Wtxn s k \<longleftrightarrow> (\<exists>t. latest_committed_wtxn s k t)"
+
+lemmas Latest_Committed_WtxnI = Latest_Committed_Wtxn_def[THEN iffD2, rule_format]
+lemmas Latest_Committed_WtxnE[elim] = Latest_Committed_Wtxn_def[THEN iffD1, elim_format, rule_format]
+         
+lemma reach_latest_committed_wtxn [simp, dest]: "reach tapir s \<Longrightarrow> Latest_Committed_Wtxn s k"
+  using T0_Committed_def[of s k] Finite_Committed_Ts_def[of s k]
+  by (auto simp add: Latest_Committed_Wtxn_def arg_max_exI)
+
 
 definition Read_Twr_Cmt where
   "Read_Twr_Cmt s k \<longleftrightarrow> (\<forall>t t_wr ts wvo.
     svr_state (svrs s k) t \<in> {read (Some t_wr),
                               prepared ts (Some t_wr) wvo,
                               committed ts (Some t_wr) wvo} \<longrightarrow> 
-    (\<exists>ts' rto' v. svr_state (svrs s k) t_wr = committed ts' rto' (Some v)))"
+    is_committed_wr (svr_state (svrs s k) t_wr))"
                                                            
 lemmas Read_Twr_CmtI = Read_Twr_Cmt_def[THEN iffD2, rule_format]
 lemmas Read_Twr_CmtE[elim] = Read_Twr_Cmt_def[THEN iffD1, elim_format, rule_format]
@@ -126,25 +167,47 @@ next
   then show ?case
   proof (induction e)
     case (Read_Resp x1 x2 x3)
-    then show ?case using Svr_Ver_Ord_Non_Emp_def[of s k] Svr_Ver_Ord_Cmt_def[of s k]
-      apply (simp add: Read_Twr_Cmt_def tapir_trans_defs)
-      by (smt last_in_set option.discI option.inject svr_state.distinct(5))
+    then show ?case
+    proof (cases "k = x1")
+      case True
+      then show ?thesis unfolding Read_Twr_Cmt_def
+      proof (intro allI)
+        fix t t_wr ts wvo
+        show "svr_state (svrs s' k) t \<in> {read (Some t_wr),
+                                         prepared ts (Some t_wr) wvo,
+                                         committed ts (Some t_wr) wvo} \<longrightarrow>
+          is_committed_wr (svr_state (svrs s' k) t_wr)"
+        proof (cases "t = Tn x2")
+          case True
+          then show ?thesis
+            using Read_Resp(1,2) \<open>k = x1\<close> Latest_Committed_Wtxn_def[of s x1]
+            apply (auto simp add: tapir_trans_defs split: if_split_asm)
+            apply (metis is_arg_max_def is_committed_wr.simps(2) some_eq_imp)
+            by (metis is_arg_max_def some_eq_imp)
+        next
+          case False
+          then show ?thesis using Read_Resp \<open>k = x1\<close>
+            apply (auto simp add: Read_Twr_Cmt_def tapir_trans_defs)
+            by (metis is_committed_wr.simps(2))+
+        qed
+      qed
+    qed (auto simp add: tapir_trans_defs Read_Twr_Cmt_def)
   next
     case (Prep x1 x2 x3 x4 x5a)
     then show ?case
       apply (auto simp add: Read_Twr_Cmt_def tapir_trans_defs)
-      apply (metis occ_check_resE svr_state.distinct(11) svr_state.distinct(17) svr_state.inject(2))
-      by (metis svr_state.distinct(11))+
+      apply (metis is_committed_wr.simps(3) occ_check_resE svr_state.distinct(17) svr_state.inject(2))
+      by (metis is_committed_wr.simps(3))+
   next
     case (Commit x1 x2 x3 x4 x5a)
     then show ?case
       apply (auto simp add: Read_Twr_Cmt_def tapir_trans_defs)
-      by (metis svr_state.distinct(15))+
+      by (metis is_committed_wr.simps(4))+
   next
     case (Abort x1 x2)
     then show ?case
       apply (simp add: Read_Twr_Cmt_def tapir_trans_defs)
-      by (metis svr_state.distinct(15) svr_state.distinct(19))
+      by (metis is_committed_wr.simps(4) is_committed_wr.simps(6))
   qed (auto simp add: Read_Twr_Cmt_def tapir_trans_defs)
 qed
 
@@ -187,7 +250,7 @@ qed
 subsection \<open>Refinement Attempt\<close>
 
 abbreviation invariants_list where                                   
-  "invariants_list s \<equiv> (\<forall>k. Svr_Ver_Ord_Non_Emp s k) \<and> (\<forall>k. Svr_Ver_Ord_Cmt s k) \<and>
+  "invariants_list s \<equiv> (\<forall>k. T0_Committed s k) \<and> (\<forall>k. Finite_Committed s k) \<and>
                       (\<forall>k. Read_Twr_Cmt s k) \<and> (\<forall>cl. CO_Tid s cl)"
 
 lemma tps_refines_et_es: "tapir \<sqsubseteq>\<^sub>med ET_SER.ET_ES"
@@ -239,7 +302,7 @@ next
             then obtain ts' rto' v where "svr_state (svrs gs k) t_wr = committed ts' rto' (Some v)"
               using cmt reach_s Read_Twr_Cmt_def[of gs]
               apply (auto simp add: cl_commit_def)
-              by (metis (no_types, lifting) Un_iff domI)
+              by (metis Un_iff domI is_committed_wr.elims(2))
             then show "F k R = Some (view_snapshot (kvs_of_s gs) u'' k)"
               using cmt \<open>r_map k = Some t_wr\<close>
               apply (auto simp add: cl_commit_def view_snapshot_def)
